add range available and helper functions etc.

VST-introduction/verif_simple_kfree_file_v2.v
@@ -8,6 +8,154 @@ Local Open Scope logic.
 
 Definition t_run := Tstruct _run noattr.
 Definition t_struct_kmem := Tstruct _struct_kmem noattr.
+Definition PGSIZE : Z := 4096. 
+
+
+(************************ Helper functions and tactics  *************************)
+
+Ltac auto_contradict := try discriminate; try contradiction.
+Ltac split_lia := split; try rep_lia.
+
+Lemma cmp_le_is_either_0_or_1 : forall p q i,
+   sem_cmp_pp Cle p q = Some (Vint i) ->
+   (i = Int.zero) \/ (i = Int.one).
+Proof.
+intros.
+destruct (eq_dec i Int.zero). left; auto.
+destruct (eq_dec i Int.one). right; auto.
+unfold sem_cmp_pp in H. inversion H.
+unfold bool2val in H1. unfold Z.b2z in H1. unfold option_map in H1.
+destruct (Val.cmplu_bool true2 Cle p q).
+- destruct b; inversion H1; exfalso.
+   + apply n0; auto.
+   + apply n; auto.
+- inversion H1.
+Qed.
+
+Lemma ptrofs_add_simpl :
+  forall a ofs,
+    0 <= ofs <= Ptrofs.max_unsigned ->
+    0 <= Ptrofs.unsigned a + ofs < Ptrofs.modulus ->
+    Ptrofs.unsigned (Ptrofs.add a (Ptrofs.repr ofs)) =
+    Ptrofs.unsigned a + ofs.
+Proof.
+  intros.
+  unfold Ptrofs.add.
+  rewrite Ptrofs.unsigned_repr.
+  - rewrite Ptrofs.unsigned_repr; auto.
+  - destruct H; assert (Ptrofs.unsigned (Ptrofs.repr ofs) = ofs). { apply Ptrofs.unsigned_repr; try rep_lia. } split.
+    + rewrite H2; try rep_lia.
+    + rewrite H2; auto; try rep_lia.
+Qed.
+
+Lemma ptrofs_unsigned_sub_self :
+  forall p : ptrofs,
+    Ptrofs.unsigned p + - Ptrofs.unsigned p = 0.
+Proof. intros p; lia. Qed.
+
+Ltac ptrofs_add_simpl_PGSIZE := apply ptrofs_add_simpl; split_lia; unfold PGSIZE; rep_lia.
+
+Lemma PGSIZE_bounds :
+   0 <= PGSIZE <= Ptrofs.max_unsigned.
+Proof. unfold PGSIZE; rep_lia. Qed.
+
+Lemma c_tmp_bounds_max:
+forall (p_s_init p_s_tmp p_n_init:ptrofs) (c_tmp:Z),
+   Ptrofs.unsigned p_s_tmp = Ptrofs.unsigned p_s_init + c_tmp * PGSIZE ->
+   0 <= c_tmp ->
+   Ptrofs.unsigned p_s_tmp <= Ptrofs.unsigned p_n_init -> 
+   Ptrofs.unsigned p_n_init + PGSIZE <= Int.max_signed  -> 
+  c_tmp + 1 <= Int.max_signed.
+Proof.
+      intros.
+      apply Z.le_trans with (m := Ptrofs.unsigned p_s_init + c_tmp * PGSIZE + PGSIZE); try rep_lia.
+      assert (Ptrofs.unsigned p_s_init + c_tmp * PGSIZE + PGSIZE = Ptrofs.unsigned p_s_init + (c_tmp + 1) * PGSIZE) by rep_lia.
+      destruct c_tmp; auto_contradict; unfold PGSIZE; auto; try rep_lia.
+Qed.
+
+Lemma c_tmp_bounds:
+forall (p_s_init p_s_tmp p_n_init:ptrofs) (c_tmp:Z),
+   Ptrofs.unsigned p_s_tmp = Ptrofs.unsigned p_s_init + c_tmp * PGSIZE ->
+   0 <= c_tmp ->
+   Ptrofs.unsigned p_s_tmp <= Ptrofs.unsigned p_n_init -> 
+   Ptrofs.unsigned p_n_init + PGSIZE <= Int.max_signed  -> 
+  Int.min_signed <= c_tmp + 1 <= Int.max_signed.
+Proof.
+      split_lia.
+      apply c_tmp_bounds_max with (p_s_init:=p_s_init) (p_s_tmp:=p_s_tmp) (p_n_init:=p_n_init); try rep_lia.
+Qed.
+
+Lemma typed_true_offset_val_leq (b_s_init b_n_init : block) 
+      (p_s_tmp p_n_init : ptrofs) (ofs : Z) :
+  typed_true tint
+    match sem_cmp_pp Cle (offset_val ofs (Vptr b_s_init p_s_tmp)) (Vptr b_n_init p_n_init) with
+    | Some v' => v'
+    | None => Vundef
+    end ->
+  Ptrofs.unsigned (Ptrofs.add p_s_tmp (Ptrofs.repr ofs)) <= Ptrofs.unsigned p_n_init.
+Proof.
+   destruct (sem_cmp_pp Cle (offset_val ofs (Vptr b_s_init p_s_tmp)) 
+   (Vptr b_n_init p_n_init)) eqn:e; auto_contradict.
+   destruct v; auto_contradict.
+   assert (i = Int.zero \/ i = Int.one). { apply cmp_le_is_either_0_or_1 with (p:= (offset_val ofs (Vptr b_s_init p_s_tmp))) (q:=(Vptr b_n_init p_n_init) ); auto. }
+   destruct H; subst; auto_contradict.
+   unfold sem_cmp_pp in e; simpl in e. destruct (eq_block b_s_init b_n_init); auto_contradict.
+   intros. subst.
+   destruct ((negb (Ptrofs.ltu p_n_init (Ptrofs.add p_s_tmp (Ptrofs.repr ofs))))) eqn:e1; auto_contradict.
+   unfold negb in e1. destruct (Ptrofs.ltu p_n_init (Ptrofs.add p_s_tmp (Ptrofs.repr ofs))) eqn:e2; auto_contradict.
+   unfold Ptrofs.ltu in e2. destruct (zlt (Ptrofs.unsigned p_n_init) (Ptrofs.unsigned (Ptrofs.add p_s_tmp (Ptrofs.repr ofs)))) eqn: e3; auto_contradict.
+   try rep_lia.
+Qed.
+
+Lemma typed_false_offset_val_leq (b_s_init b_n_init : block) 
+      (p_s_tmp p_n_init : ptrofs) (ofs : Z) :
+   Ptrofs.unsigned p_s_tmp + ofs < Ptrofs.modulus -> (* I know the ofs =PGSIZE*)
+   0 <= ofs <= Ptrofs.max_unsigned ->
+   typed_false tint
+      match sem_cmp_pp Cle (offset_val ofs (Vptr b_s_init p_s_tmp)) (Vptr b_n_init p_n_init) with
+      | Some v' => v'
+      | None => Vundef
+      end ->
+   Ptrofs.unsigned p_n_init < Ptrofs.unsigned p_s_tmp + ofs.
+Proof.
+   destruct (sem_cmp_pp Cle (offset_val ofs (Vptr b_s_init p_s_tmp)) 
+   (Vptr b_n_init p_n_init)) eqn:e; auto_contradict.
+   destruct v; auto_contradict.
+   assert (i = Int.zero \/ i = Int.one). { apply cmp_le_is_either_0_or_1 with (p:= (offset_val ofs (Vptr b_s_init p_s_tmp))) (q:=(Vptr b_n_init p_n_init) ); auto. }
+   destruct H; subst; auto_contradict.
+   subst. unfold sem_cmp_pp in e. simpl in e. destruct (eq_block b_s_init b_n_init); auto_contradict.
+   destruct ((negb (Ptrofs.ltu p_n_init (Ptrofs.add p_s_tmp (Ptrofs.repr ofs))))) eqn:e1; auto_contradict.
+   unfold negb in e1; unfold Ptrofs.ltu in e1. destruct (zlt (Ptrofs.unsigned p_n_init) (Ptrofs.unsigned (Ptrofs.add p_s_tmp (Ptrofs.repr ofs)))) eqn:e2; auto_contradict.
+   intros.
+   assert (Ptrofs.unsigned (Ptrofs.add p_s_tmp (Ptrofs.repr ofs)) = Ptrofs.unsigned p_s_tmp + ofs) by ptrofs_add_simpl_PGSIZE.
+   rewrite <- H2. unfold PGSIZE; apply l.
+Qed.
+
+(* solves something like "0 <= a + - a + b" *)
+Ltac le_sub_self_add_and_solve :=
+  rewrite ptrofs_unsigned_sub_self;
+  apply Z.add_nonneg_nonneg;
+  unfold PGSIZE;
+  rep_lia.
+
+Lemma sameblock_true :
+forall b_s_init b_n_init p_s_tmp p_n_init,
+   sameblock (Vptr b_s_init p_s_tmp) (Vptr b_n_init p_n_init) = true ->
+   b_s_init = b_n_init.
+Proof.
+   intros. unfold sameblock in H.
+   destruct (peq b_s_init b_n_init); try rep_lia; auto_contradict.
+Qed.
+
+Lemma sameblock_eq_false :
+forall b_s_init b_n_init p_s_tmp p_n_init,
+   sameblock (Vptr b_s_init p_s_tmp) (Vptr b_n_init p_n_init) = false ->
+   b_s_init <> b_n_init.
+Proof.
+   intros. unfold sameblock in H.
+   destruct (peq b_s_init b_n_init); try rep_lia; auto_contradict.
+Qed.
+
 
 (************** pointer comparison **************'*)
 
@@ -50,7 +198,7 @@ Proof.
 Lemma freelistrep_valid_pointer:
   forall sh n p, 
   readable_share sh ->
-   freelistrep Ews n p |-- valid_pointer p.
+   freelistrep sh n p |-- valid_pointer p.
 Proof.
   intros. destruct n.
   - unfold freelistrep. entailer!.
@@ -86,7 +234,180 @@ Proof.
    - Intros m y. rewrite H0. unfold freelistrep at 2; fold freelistrep. Exists y. entailer!.
 Qed.
 
-Definition kfree1_freelist_spec := 
+
+
+(****************** range available *********************)
+
+Definition compute_c (p_start p_end: val) (size: Z) : Z :=
+   match p_start, p_end with
+   |  Vptr b1 p1 , Vptr b2 p2 =>
+         if (size <=? 0)%Z then 0 (* Avoid division by zero *)
+         else if (Ptrofs.ltu p2 p1) then 0 (* we don't want p2 < p1, meaning we have p1 <= p2, when we have a real result *)
+         else
+          (Ptrofs.unsigned p2 - Ptrofs.unsigned p1) / size (* take the floor *)
+   | _ , _ => 0
+   end.
+(*Compute (compute_c (Vptr (Block.repr 0) (Ptrofs.repr 1000)) (Vptr 0 (Ptrofs.repr 5000)) 4096).*)
+
+Definition add_offset (p: val) (ofs: Z) : val := 
+   match p with
+   | Vptr b1 p1 => Vptr b1 (Ptrofs.add p1 (Ptrofs.repr ofs))
+   | _ => nullval
+   end.
+
+(*Definition sub_pointers (p_1 p_2: val) : val := 
+   match p_1, p_2 with
+   | Vptr b1 p1 , Vptr b2 p2 => if (sameblock p_1 p_2) then (Vptr b1 (Ptrofs.sub p1 p2)) else nullval
+   | _, _ => nullval
+   end.*)
+
+Fixpoint available (sh: share) (n: nat) (p: val) (size: Z) : mpred :=
+  match n with
+  | S n' => 
+      !! malloc_compatible (sizeof t_run) p &&  (* Check memory compatibility *)
+      data_at sh t_run nullval p *            (* Store null value *)
+      available sh n' (add_offset p size) size (* Move to the next slot *)
+  | O => !! (p = nullval) && emp
+  end.
+
+Definition available_range (sh: share) (p_start p_end: val) (size: Z) :=
+   match p_start, p_end with
+   | Vptr b_s p_s, Vptr b_e p_e =>
+      if (sameblock p_start p_end) then
+         available sh (Z.to_nat (compute_c p_start p_end size)) p_start size
+      else !! (p_start = nullval) && emp
+   | _ , _ => !! (p_start = nullval) && emp
+   end.
+
+Arguments available_range sh p_start p_end size : simpl never.
+
+
+Lemma available_local_prop: forall sh n p size, 
+   available sh n p size |--  !! (is_pointer_or_null p /\ (n=0<->p=nullval) /\ (n>0<->isptr p))%nat.
+Proof.
+  intros.
+  induction n as [| n' IH].
+  - unfold available. entailer!. split; auto.
+    + split; auto.
+    + split; try lia. intros. simpl in *. inversion H.
+  - unfold available. destruct p; entailer!. split; split; intros; try rep_lia; auto; auto_contradict.
+   Qed.
+#[export] Hint Resolve available_local_prop : saturate_local.
+
+
+Lemma available_valid_pointer:
+  forall sh n p size, 
+  readable_share sh ->
+   available sh n p size |-- valid_pointer p.
+Proof.
+  intros. destruct n.
+  - unfold available. entailer!.
+  - unfold available. entailer.
+Qed. 
+#[export] Hint Resolve available_valid_pointer : valid_pointer.
+
+Lemma available_null: forall sh n x size,
+       x = nullval ->
+       available sh n x size = !! (n = O) && emp.
+Proof.
+   intros.
+   destruct n; unfold available; fold available.
+   autorewrite with norm. auto.
+   apply pred_ext.
+   entailer. 
+   destruct n; entailer!; try discriminate H0. 
+Qed.
+
+Lemma available_nonnull: forall n sh x size,
+   x <> nullval ->
+   available sh n x size =
+   EX m : nat, 
+          !! (n = S m) && !! malloc_compatible (sizeof t_run) x && data_at sh t_run nullval x * available sh m (add_offset x size) size.
+Proof.
+   intros; apply pred_ext.
+   - destruct n. 
+         + unfold available. entailer!.
+         + unfold available; fold available.
+         Exists n. entailer!.
+   - Intros m. rewrite H0. unfold available at 2; fold available. entailer!.
+Qed.
+
+
+(** lemmas ***)
+Lemma available_0:
+  forall sh p size, available sh 0 p size = !! (p = nullval) && emp.
+Proof.
+  intros. simpl. reflexivity.
+Qed.
+
+Lemma available_S:
+  forall sh n p size,
+    available sh (S n) p size =
+    !! malloc_compatible (sizeof t_run) p &&
+    data_at sh t_run nullval p * available sh n (add_offset p size) size.
+Proof.
+  intros. simpl. reflexivity.
+Qed.
+
+
+Lemma add_offset_correct:
+  forall b p size,
+    add_offset (Vptr b p) size = Vptr b (Ptrofs.add p (Ptrofs.repr size)).
+Proof.
+  intros. unfold add_offset. reflexivity.
+Qed.
+
+
+Lemma compute_c_correct1:
+  forall b (p1 p2: ptrofs) size,
+   (*0 < size ->
+    Ptrofs.unsigned p1 <= Ptrofs.unsigned p2 -> *)
+    0 < size ->
+    Ptrofs.unsigned p1 <= Ptrofs.unsigned p2 ->
+    Ptrofs.unsigned p1 + (compute_c (Vptr b p1) (Vptr b p2) size) <= Ptrofs.unsigned p2.
+Proof.
+  intros. unfold compute_c. Admitted.
+
+(* p1 + c + ? = p2 
+   ? <= size
+   ? = p2 - (p1 + c)
+   p2 - (p1 + c) <= size
+*)
+
+Lemma compute_c_correct2:
+  forall b (p1 p2: ptrofs) size,
+    0 < size ->
+    Ptrofs.unsigned p1 <= Ptrofs.unsigned p2 ->
+    (Ptrofs.unsigned p2 - (Ptrofs.unsigned p1 + (compute_c (Vptr b p1) (Vptr b p2) size))) <= size.
+Proof.
+  intros. unfold compute_c.
+  destruct (size <=? 0) eqn:e; try rep_lia.
+  unfold Ptrofs.ltu.
+  destruct (Ptrofs.ltu p1 p2) eqn:e2; unfold Ptrofs.ltu in e2; destruct (zlt (Ptrofs.unsigned p1) (Ptrofs.unsigned p2)) eqn:e3; try rep_lia; auto_contradict.
+  + destruct (zlt (Ptrofs.unsigned p2) (Ptrofs.unsigned p1)); try rep_lia. admit.
+  + assert (Ptrofs.unsigned p1 = Ptrofs.unsigned p2); try rep_lia.
+   rewrite H1. destruct (zlt (Ptrofs.unsigned p2) (Ptrofs.unsigned p2)); try rep_lia.
+   assert (Ptrofs.unsigned p2 - Ptrofs.unsigned p2 = 0) by rep_lia.
+   rewrite H2; rewrite Z.add_0_r. try rep_lia.
+Admitted.
+
+
+Lemma available_range_correct:
+  forall sh p_start p_end size,
+    available_range sh p_start p_end size |-- available sh (Z.to_nat (compute_c p_start p_end size)) p_start size.
+Proof.
+  intros.
+  unfold available_range.
+  destruct p_start, p_end; try apply derives_refl.
+  destruct (sameblock (Vptr b i) (Vptr b0 i0)); entailer; auto_contradict.
+Qed.
+
+
+
+(************************ specs *********************************)
+
+
+(*Definition kfree1_freelist_spec := 
    DECLARE _kfree1
       WITH sh : share, new_head:val, original_freelist_pointer:val, xx:Z, gv:globals, n : nat
       PRE [ tptr tvoid]
@@ -96,6 +417,25 @@ Definition kfree1_freelist_spec :=
             freelistrep sh n original_freelist_pointer *
             (!! malloc_compatible (sizeof t_run) new_head &&
             data_at sh (t_run) nullval new_head *
+            data_at sh t_struct_kmem (Vint (Int.repr xx), original_freelist_pointer) (gv _kmem) )
+         )
+      POST [ tvoid ]
+         PROP()
+         RETURN () 
+         SEP (
+            freelistrep sh (S n) new_head *
+            data_at sh t_struct_kmem (Vint (Int.repr xx), new_head) (gv _kmem)
+            ).*)
+Definition kfree1_freelist_spec := 
+   DECLARE _kfree1
+      WITH sh : share, new_head:val, original_freelist_pointer:val, xx:Z, gv:globals, n : nat, size:Z
+      PRE [ tptr tvoid]
+         PROP(writable_share sh; is_pointer_or_null original_freelist_pointer) 
+         PARAMS (new_head) GLOBALS(gv)
+         SEP (
+            freelistrep sh n original_freelist_pointer *
+            available sh (S O) new_head PGSIZE *
+            (
             data_at sh t_struct_kmem (Vint (Int.repr xx), original_freelist_pointer) (gv _kmem) )
          )
       POST [ tvoid ]
@@ -140,7 +480,7 @@ Definition freerange_no_loop_no_add_spec :=
          ).
 
 (************** pointer comparison add + call **************'*)
-Definition PGSIZE : Z := 4096. 
+
 
 Definition freerange_no_loop_no_add_1_spec :=
    DECLARE _freerange_no_loop_no_add_1
@@ -185,14 +525,11 @@ Definition while_1_5_spec : ident * funspec := (* this is not including admits..
             ) (* the highest number is s + PGSIZE when it fails. The highest s + PGSIZE when it succeeds is n, so the highest after this is n + PGSIZE*)
         PARAMS (Vptr b_s_init p_s_init; Vptr b_n_init p_n_init)
         SEP (
-         denote_tc_test_order (Vptr b_s_init (Ptrofs.add p_s_init (Ptrofs.repr PGSIZE)))
-                                  (Vptr b_n_init p_n_init) &&
+         denote_tc_test_order (Vptr b_s_init (Ptrofs.add p_s_init (Ptrofs.repr PGSIZE))) (Vptr b_n_init p_n_init) &&
          (!! (forall p_s_tmp,
-         Ptrofs.unsigned p_s_init <= Ptrofs.unsigned p_s_tmp <= Ptrofs.unsigned p_n_init ->
-         ((denote_tc_test_order (Vptr b_s_init (Ptrofs.add p_s_tmp (Ptrofs.repr PGSIZE)))
-         (Vptr b_n_init p_n_init)) |--
-            (denote_tc_test_order (Vptr b_s_init (Ptrofs.add p_s_tmp (Ptrofs.repr (PGSIZE + PGSIZE))))
-                                  (Vptr b_n_init p_n_init)))
+            Ptrofs.unsigned p_s_init <= Ptrofs.unsigned p_s_tmp <= Ptrofs.unsigned p_n_init ->
+            (denote_tc_test_order (Vptr b_s_init (Ptrofs.add p_s_tmp (Ptrofs.repr PGSIZE))) (Vptr b_n_init p_n_init)) 
+               |-- (denote_tc_test_order (Vptr b_s_init (Ptrofs.add p_s_tmp (Ptrofs.repr (PGSIZE + PGSIZE)))) (Vptr b_n_init p_n_init))
          ))
         )
     POST [ tint ]
@@ -216,26 +553,147 @@ Definition freerange_while_loop_spec : ident * funspec := (* this is not includi
         PROP (
                 0 <= Ptrofs.unsigned p_s_init <= Ptrofs.unsigned p_n_init /\
                 Z.add (Ptrofs.unsigned p_n_init) PGSIZE <= Int.max_signed /\ 
-                Z.add (Ptrofs.unsigned p_s_init) PGSIZE <= Int.max_signed 
+                Z.add (Ptrofs.unsigned p_s_init) PGSIZE <= Int.max_signed /\
+
+                writable_share sh /\
+                is_pointer_or_null original_freelist_pointer 
+
             ) (* the highest number is s + PGSIZE when it fails. The highest s + PGSIZE when it succeeds is n, so the highest after this is n + PGSIZE*)
         PARAMS (Vptr b_s_init p_s_init; Vptr b_n_init p_n_init) GLOBALS (gv)
         SEP (
-         denote_tc_test_order (Vptr b_s_init (Ptrofs.add p_s_init (Ptrofs.repr PGSIZE))) (Vptr b_n_init p_n_init) &&
+         (denote_tc_test_order (Vptr b_s_init (Ptrofs.add p_s_init (Ptrofs.repr PGSIZE))) (Vptr b_n_init p_n_init) &&
          (!! (forall p_s_tmp,
+            Ptrofs.unsigned p_s_init <= Ptrofs.unsigned p_s_tmp <= Ptrofs.unsigned p_n_init ->
+            (denote_tc_test_order (Vptr b_s_init (Ptrofs.add p_s_tmp (Ptrofs.repr PGSIZE))) (Vptr b_n_init p_n_init)) 
+               |-- (denote_tc_test_order (Vptr b_s_init (Ptrofs.add p_s_tmp (Ptrofs.repr (PGSIZE + PGSIZE)))) (Vptr b_n_init p_n_init))
+         )))
+         &&
+         (((freelistrep sh n original_freelist_pointer (*&&
+            (!! forall p_s_tmp, Ptrofs.unsigned p_s_init <= Ptrofs.unsigned p_s_tmp + PGSIZE <= Ptrofs.unsigned p_n_init -> 
+               freelistrep sh n (Vptr b_s_init p_s_tmp) |-- freelistrep sh (S n) (Vptr b_s_init (Ptrofs.add p_s_tmp (Ptrofs.repr PGSIZE))))*))
+            * available_range sh (Vptr b_s_init p_s_init) (Vptr b_n_init p_n_init) (compute_c (Vptr b_s_init p_s_init) (Vptr b_n_init p_n_init) PGSIZE)
+            * (data_at sh t_struct_kmem (Vint (Int.repr xx), original_freelist_pointer) (gv _kmem))
+               (*((data_at sh t_struct_kmem (Vint (Int.repr xx), original_freelist_pointer) (gv _kmem)) &&
+               ((!! forall p_s_tmp, Ptrofs.unsigned p_s_init <= Ptrofs.unsigned p_s_tmp + PGSIZE <= Ptrofs.unsigned p_n_init -> 
+                  (data_at sh t_struct_kmem (Vint (Int.repr xx), (Vptr b_s_init p_s_init)) (gv _kmem)) |-- 
+                  (data_at sh t_struct_kmem (Vint (Int.repr xx), (Vptr b_s_init (Ptrofs.add p_s_tmp (Ptrofs.repr PGSIZE)))) (gv _kmem))))
+         )*))))
+    POST [ tvoid ]
+    EX c_final:Z, EX p_s_final:ptrofs,
+        PROP (
+            Ptrofs.unsigned p_s_final = Z.add (Ptrofs.unsigned p_s_init) (Z.mul c_final PGSIZE) /\ 
+            0 <= c_final /\ 
+            (Ptrofs.unsigned p_s_final) <= (Ptrofs.unsigned p_n_init) /\ 
+            (Ptrofs.unsigned p_n_init) < Z.add (Ptrofs.unsigned p_s_final) PGSIZE
+            )
+        RETURN ()
+        SEP (denote_tc_test_order (Vptr b_s_init (Ptrofs.add p_s_final (Ptrofs.repr PGSIZE))) (Vptr b_n_init p_n_init) &&
+               (freelistrep sh (Nat.add (Z.to_nat c_final) n) (Vptr b_s_init p_s_final) *
+               data_at sh t_struct_kmem (Vint (Int.repr xx), (Vptr b_s_init p_s_final)) (gv _kmem))
+        ).
+
+
+
+
+(*Definition freerange_while_loop_spec : ident * funspec := (* this is not including admits.. *)
+    DECLARE _freerange_while_loop
+    WITH b_n_init:block, p_n_init:ptrofs, b_s_init:block, p_s_init:ptrofs, 
+            sh : share, original_freelist_pointer : val, xx : Z, gv : globals, n:nat
+    PRE [  tptr tvoid, tptr tvoid ]
+        PROP (
+                0 <= Ptrofs.unsigned p_s_init <= Ptrofs.unsigned p_n_init /\
+                Z.add (Ptrofs.unsigned p_n_init) PGSIZE <= Int.max_signed /\ 
+                Z.add (Ptrofs.unsigned p_s_init) PGSIZE <= Int.max_signed /\
+
+                writable_share sh /\
+                is_pointer_or_null original_freelist_pointer 
+
+            ) (* the highest number is s + PGSIZE when it fails. The highest s + PGSIZE when it succeeds is n, so the highest after this is n + PGSIZE*)
+        PARAMS (Vptr b_s_init p_s_init; Vptr b_n_init p_n_init) GLOBALS (gv)
+        SEP (
+         (denote_tc_test_order (Vptr b_s_init (Ptrofs.add p_s_init (Ptrofs.repr PGSIZE))) (Vptr b_n_init p_n_init) &&
+         (!! (forall p_s_tmp,
+            Ptrofs.unsigned p_s_init <= Ptrofs.unsigned p_s_tmp <= Ptrofs.unsigned p_n_init ->
+            (denote_tc_test_order (Vptr b_s_init (Ptrofs.add p_s_tmp (Ptrofs.repr PGSIZE))) (Vptr b_n_init p_n_init)) 
+               |-- (denote_tc_test_order (Vptr b_s_init (Ptrofs.add p_s_tmp (Ptrofs.repr (PGSIZE + PGSIZE)))) (Vptr b_n_init p_n_init))
+         )))
+         &&
+         (((freelistrep sh n original_freelist_pointer (*&&
+            (!! forall p_s_tmp, Ptrofs.unsigned p_s_init <= Ptrofs.unsigned p_s_tmp + PGSIZE <= Ptrofs.unsigned p_n_init -> 
+               freelistrep sh n (Vptr b_s_init p_s_tmp) |-- freelistrep sh (S n) (Vptr b_s_init (Ptrofs.add p_s_tmp (Ptrofs.repr PGSIZE))))*))
+            *
+            ((!! forall p_s_tmp, Ptrofs.unsigned p_s_init <= Ptrofs.unsigned p_s_tmp <= Ptrofs.unsigned p_n_init -> 
+               malloc_compatible (sizeof t_run) (Vptr b_s_init p_s_tmp))
+               &&
+               (data_at sh (t_run) nullval (Vptr b_s_init p_s_init) &&
+               (!! (forall p_s_tmp,
                   Ptrofs.unsigned p_s_init <= Ptrofs.unsigned p_s_tmp <= Ptrofs.unsigned p_n_init ->
-                  ((denote_tc_test_order (Vptr b_s_init (Ptrofs.add p_s_tmp (Ptrofs.repr PGSIZE))) (Vptr b_n_init p_n_init)) |--
-                     (denote_tc_test_order (Vptr b_s_init (Ptrofs.add p_s_tmp (Ptrofs.repr (PGSIZE + PGSIZE)))) (Vptr b_n_init p_n_init)))
-         )) &&
-         (freelistrep sh n original_freelist_pointer *
-         ((!! forall p_s_tmp, Ptrofs.unsigned p_s_init <= Ptrofs.unsigned p_s_tmp <= Ptrofs.unsigned p_n_init -> 
-             malloc_compatible (sizeof t_run) (Vptr b_s_init p_s_tmp)) &&
+                  data_at sh (t_run) nullval (Vptr b_s_init p_s_tmp) |--
+                  data_at sh (t_run) nullval (Vptr b_s_init (Ptrofs.add p_s_tmp (Ptrofs.repr PGSIZE)))
+                  )))
+               *
+               ((data_at sh t_struct_kmem (Vint (Int.repr xx), original_freelist_pointer) (gv _kmem)) &&
+               ((!! forall p_s_tmp, Ptrofs.unsigned p_s_init <= Ptrofs.unsigned p_s_tmp + PGSIZE <= Ptrofs.unsigned p_n_init -> 
+                  (data_at sh t_struct_kmem (Vint (Int.repr xx), (Vptr b_s_init p_s_init)) (gv _kmem)) |-- 
+                  (data_at sh t_struct_kmem (Vint (Int.repr xx), (Vptr b_s_init (Ptrofs.add p_s_tmp (Ptrofs.repr PGSIZE)))) (gv _kmem))))
+         )))))
+    POST [ tvoid ]
+    EX c_final:Z, EX p_s_final:ptrofs,
+        PROP (
+            Ptrofs.unsigned p_s_final = Z.add (Ptrofs.unsigned p_s_init) (Z.mul c_final PGSIZE) /\ 
+            0 <= c_final /\ 
+            (Ptrofs.unsigned p_s_final) <= (Ptrofs.unsigned p_n_init) /\ 
+            (Ptrofs.unsigned p_n_init) < Z.add (Ptrofs.unsigned p_s_final) PGSIZE
+            )
+        RETURN ()
+        SEP (denote_tc_test_order (Vptr b_s_init (Ptrofs.add p_s_final (Ptrofs.repr PGSIZE))) (Vptr b_n_init p_n_init) &&
+               (freelistrep sh (Nat.add (Z.to_nat c_final) n) (Vptr b_s_init p_s_final) *
+               data_at sh t_struct_kmem (Vint (Int.repr xx), (Vptr b_s_init p_s_final)) (gv _kmem))
+        ).*)
+
+(*
+Definition freerange_while_loop_spec : ident * funspec := (* this is not including admits.. *)
+    DECLARE _freerange_while_loop
+    WITH b_n_init:block, p_n_init:ptrofs, b_s_init:block, p_s_init:ptrofs, 
+            sh : share, original_freelist_pointer : val, xx : Z, gv : globals, n:nat
+    PRE [  tptr tvoid, tptr tvoid ]
+        PROP (
+                0 <= Ptrofs.unsigned p_s_init <= Ptrofs.unsigned p_n_init /\
+                Z.add (Ptrofs.unsigned p_n_init) PGSIZE <= Int.max_signed /\ 
+                Z.add (Ptrofs.unsigned p_s_init) PGSIZE <= Int.max_signed /\
+
+                writable_share sh /\
+                is_pointer_or_null original_freelist_pointer 
+
+            ) (* the highest number is s + PGSIZE when it fails. The highest s + PGSIZE when it succeeds is n, so the highest after this is n + PGSIZE*)
+        PARAMS (Vptr b_s_init p_s_init; Vptr b_n_init p_n_init) GLOBALS (gv)
+        SEP (
+         (denote_tc_test_order (Vptr b_s_init (Ptrofs.add p_s_init (Ptrofs.repr PGSIZE))) (Vptr b_n_init p_n_init) &&
          (!! (forall p_s_tmp,
-             Ptrofs.unsigned p_s_init <= Ptrofs.unsigned p_s_tmp <= Ptrofs.unsigned p_n_init ->
-             data_at sh (t_run) nullval (Vptr b_s_init p_s_tmp) |--
-             data_at sh (t_run) nullval (Vptr b_s_init (Ptrofs.add p_s_tmp (Ptrofs.repr PGSIZE)))
-         )) *
-         data_at sh t_struct_kmem (Vint (Int.repr xx), original_freelist_pointer) (gv _kmem) ))
-        )
+            Ptrofs.unsigned p_s_init <= Ptrofs.unsigned p_s_tmp <= Ptrofs.unsigned p_n_init ->
+            (denote_tc_test_order (Vptr b_s_init (Ptrofs.add p_s_tmp (Ptrofs.repr PGSIZE))) (Vptr b_n_init p_n_init)) 
+               |-- (denote_tc_test_order (Vptr b_s_init (Ptrofs.add p_s_tmp (Ptrofs.repr (PGSIZE + PGSIZE)))) (Vptr b_n_init p_n_init))
+         )))
+         &&
+         (((freelistrep sh n original_freelist_pointer &&
+            (!! forall p_s_tmp, Ptrofs.unsigned p_s_init <= Ptrofs.unsigned p_s_tmp + PGSIZE <= Ptrofs.unsigned p_n_init -> 
+               freelistrep sh n (Vptr b_s_init p_s_tmp) |-- freelistrep sh (S n) (Vptr b_s_init (Ptrofs.add p_s_tmp (Ptrofs.repr PGSIZE)))))
+            *
+            ((!! forall p_s_tmp, Ptrofs.unsigned p_s_init <= Ptrofs.unsigned p_s_tmp <= Ptrofs.unsigned p_n_init -> 
+               malloc_compatible (sizeof t_run) (Vptr b_s_init p_s_tmp))
+               &&
+               (data_at sh (t_run) nullval (Vptr b_s_init p_s_init) &&
+               (!! (forall p_s_tmp,
+                  Ptrofs.unsigned p_s_init <= Ptrofs.unsigned p_s_tmp <= Ptrofs.unsigned p_n_init ->
+                  data_at sh (t_run) nullval (Vptr b_s_init p_s_tmp) |--
+                  data_at sh (t_run) nullval (Vptr b_s_init (Ptrofs.add p_s_tmp (Ptrofs.repr PGSIZE)))
+                  )))
+               *
+               ((data_at sh t_struct_kmem (Vint (Int.repr xx), original_freelist_pointer) (gv _kmem)) &&
+               ((!! forall p_s_tmp, Ptrofs.unsigned p_s_init <= Ptrofs.unsigned p_s_tmp + PGSIZE <= Ptrofs.unsigned p_n_init -> 
+                  (data_at sh t_struct_kmem (Vint (Int.repr xx), (Vptr b_s_init p_s_init)) (gv _kmem)) |-- 
+                  (data_at sh t_struct_kmem (Vint (Int.repr xx), (Vptr b_s_init (Ptrofs.add p_s_tmp (Ptrofs.repr PGSIZE)))) (gv _kmem))))
+         )))))
     POST [ tvoid ]
     EX c:Z, EX p_s_final:ptrofs,
         PROP (
@@ -250,6 +708,7 @@ Definition freerange_while_loop_spec : ident * funspec := (* this is not includi
                data_at sh t_struct_kmem (Vint (Int.repr xx), (Vptr b_s_init p_s_final)) (gv _kmem))
         ).
 
+*)
 
 (************************ Gprog  *************************)
 Definition Gprog : funspecs := [
@@ -259,126 +718,10 @@ Definition Gprog : funspecs := [
    while_1_5_spec; freerange_while_loop_spec
 ].
 
-(************************ Helper functions and tactics  *************************)
-
-Ltac auto_contradict := try discriminate; try contradiction.
-Ltac split_lia := split; try rep_lia.
-
-Lemma cmp_le_is_either_0_or_1 : forall p q i,
-   sem_cmp_pp Cle p q = Some (Vint i) ->
-   (i = Int.zero) \/ (i = Int.one).
-Proof.
-intros.
-destruct (eq_dec i Int.zero). left; auto.
-destruct (eq_dec i Int.one). right; auto.
-unfold sem_cmp_pp in H. inversion H.
-unfold bool2val in H1. unfold Z.b2z in H1. unfold option_map in H1.
-destruct (Val.cmplu_bool true2 Cle p q).
-- destruct b; inversion H1; exfalso.
-   + apply n0; auto.
-   + apply n; auto.
-- inversion H1.
-Qed.
-
-Lemma ptrofs_add_simpl :
-  forall a ofs,
-    0 <= ofs <= Ptrofs.max_unsigned ->
-    0 <= Ptrofs.unsigned a + ofs < Ptrofs.modulus ->
-    Ptrofs.unsigned (Ptrofs.add a (Ptrofs.repr ofs)) =
-    Ptrofs.unsigned a + ofs.
-Proof.
-  intros.
-  unfold Ptrofs.add.
-  rewrite Ptrofs.unsigned_repr.
-  - rewrite Ptrofs.unsigned_repr; auto.
-  - destruct H; assert (Ptrofs.unsigned (Ptrofs.repr ofs) = ofs). { apply Ptrofs.unsigned_repr; try rep_lia. } split.
-    + rewrite H2; try rep_lia.
-    + rewrite H2; auto; try rep_lia.
-Qed.
-
-Ltac ptrofs_add_simpl_PGSIZE := apply ptrofs_add_simpl; split_lia; unfold PGSIZE; rep_lia.
-
-Lemma PGSIZE_bounds :
-   0 <= PGSIZE <= Ptrofs.max_unsigned.
-Proof. unfold PGSIZE; rep_lia. Qed.
-
-Lemma c_tmp_bounds_max:
-forall (p_s_init p_s_tmp p_n_init:ptrofs) (c_tmp:Z),
-   Ptrofs.unsigned p_s_tmp = Ptrofs.unsigned p_s_init + c_tmp * PGSIZE ->
-   0 <= c_tmp ->
-   Ptrofs.unsigned p_s_tmp <= Ptrofs.unsigned p_n_init -> 
-   Ptrofs.unsigned p_n_init + PGSIZE <= Int.max_signed  -> 
-  c_tmp + 1 <= Int.max_signed.
-Proof.
-      intros.
-      apply Z.le_trans with (m := Ptrofs.unsigned p_s_init + c_tmp * PGSIZE + PGSIZE); try rep_lia.
-      assert (Ptrofs.unsigned p_s_init + c_tmp * PGSIZE + PGSIZE = Ptrofs.unsigned p_s_init + (c_tmp + 1) * PGSIZE) by rep_lia.
-      destruct c_tmp; auto_contradict; unfold PGSIZE; auto; try rep_lia.
-Qed.
-
-Lemma c_tmp_bounds:
-forall (p_s_init p_s_tmp p_n_init:ptrofs) (c_tmp:Z),
-   Ptrofs.unsigned p_s_tmp = Ptrofs.unsigned p_s_init + c_tmp * PGSIZE ->
-   0 <= c_tmp ->
-   Ptrofs.unsigned p_s_tmp <= Ptrofs.unsigned p_n_init -> 
-   Ptrofs.unsigned p_n_init + PGSIZE <= Int.max_signed  -> 
-  Int.min_signed <= c_tmp + 1 <= Int.max_signed.
-Proof.
-      split_lia.
-      apply c_tmp_bounds_max with (p_s_init:=p_s_init) (p_s_tmp:=p_s_tmp) (p_n_init:=p_n_init); try rep_lia.
-Qed.
-
-Lemma typed_true_offset_val_leq (b_s_init b_n_init : block) 
-      (p_s_tmp p_n_init : ptrofs) (ofs : Z) :
-  typed_true tint
-    match sem_cmp_pp Cle (offset_val ofs (Vptr b_s_init p_s_tmp)) (Vptr b_n_init p_n_init) with
-    | Some v' => v'
-    | None => Vundef
-    end ->
-  Ptrofs.unsigned (Ptrofs.add p_s_tmp (Ptrofs.repr ofs)) <= Ptrofs.unsigned p_n_init.
-Proof.
-   destruct (sem_cmp_pp Cle (offset_val ofs (Vptr b_s_init p_s_tmp)) (* find a solution for magic number 4096 *)
-   (Vptr b_n_init p_n_init)) eqn:e; auto_contradict.
-   destruct v; auto_contradict.
-   assert (i = Int.zero \/ i = Int.one). { apply cmp_le_is_either_0_or_1 with (p:= (offset_val ofs (Vptr b_s_init p_s_tmp))) (q:=(Vptr b_n_init p_n_init) ); auto. }
-   destruct H; subst; auto_contradict.
-   unfold sem_cmp_pp in e; simpl in e. destruct (eq_block b_s_init b_n_init); auto_contradict.
-   intros. subst.
-   destruct ((negb (Ptrofs.ltu p_n_init (Ptrofs.add p_s_tmp (Ptrofs.repr ofs))))) eqn:e1; auto_contradict.
-   unfold negb in e1. destruct (Ptrofs.ltu p_n_init (Ptrofs.add p_s_tmp (Ptrofs.repr ofs))) eqn:e2; auto_contradict.
-   unfold Ptrofs.ltu in e2. destruct (zlt (Ptrofs.unsigned p_n_init) (Ptrofs.unsigned (Ptrofs.add p_s_tmp (Ptrofs.repr ofs)))) eqn: e3; auto_contradict.
-   try rep_lia.
-Qed.
-
-Lemma typed_false_offset_val_leq (b_s_init b_n_init : block) 
-      (p_s_tmp p_n_init : ptrofs) (ofs : Z) :
-   Ptrofs.unsigned p_s_tmp + ofs < Ptrofs.modulus -> (* I know the ofs =PGSIZE*)
-   0 <= ofs <= Ptrofs.max_unsigned ->
-   typed_false tint
-      match sem_cmp_pp Cle (offset_val ofs (Vptr b_s_init p_s_tmp)) (Vptr b_n_init p_n_init) with
-      | Some v' => v'
-      | None => Vundef
-      end ->
-   Ptrofs.unsigned p_n_init < Ptrofs.unsigned p_s_tmp + ofs.
-Proof.
-   destruct (sem_cmp_pp Cle (offset_val ofs (Vptr b_s_init p_s_tmp)) (* find a solution for magic number 4096 *)
-   (Vptr b_n_init p_n_init)) eqn:e; auto_contradict.
-   destruct v; auto_contradict.
-   assert (i = Int.zero \/ i = Int.one). { apply cmp_le_is_either_0_or_1 with (p:= (offset_val ofs (Vptr b_s_init p_s_tmp))) (q:=(Vptr b_n_init p_n_init) ); auto. }
-   destruct H; subst; auto_contradict.
-   subst. unfold sem_cmp_pp in e. simpl in e. destruct (eq_block b_s_init b_n_init); auto_contradict.
-   destruct ((negb (Ptrofs.ltu p_n_init (Ptrofs.add p_s_tmp (Ptrofs.repr ofs))))) eqn:e1; auto_contradict.
-   unfold negb in e1; unfold Ptrofs.ltu in e1. destruct (zlt (Ptrofs.unsigned p_n_init) (Ptrofs.unsigned (Ptrofs.add p_s_tmp (Ptrofs.repr ofs)))) eqn:e2; auto_contradict.
-   intros.
-   assert (Ptrofs.unsigned (Ptrofs.add p_s_tmp (Ptrofs.repr ofs)) = Ptrofs.unsigned p_s_tmp + ofs) by ptrofs_add_simpl_PGSIZE.
-   rewrite <- H2. unfold PGSIZE; apply l.
-Qed.
-
-
 
 (************************ Proofs  *************************)
 
-Lemma body_kfree1_freelist': semax_body Vprog Gprog f_kfree1 kfree1_freelist_spec.
+(*Lemma body_kfree1_freelist': semax_body Vprog Gprog f_kfree1 kfree1_freelist_spec.
 Proof. start_function. Intros. repeat forward. entailer. 
        induction n. 
        - assert (original_freelist_pointer = nullval). {
@@ -387,9 +730,20 @@ Proof. start_function. Intros. repeat forward. entailer.
          rewrite H7. unfold freelistrep. Exists nullval. entailer.
       - unfold freelistrep. Intros next_orig. Exists original_freelist_pointer. entailer.
          Exists next_orig. entailer. fold freelistrep. entailer!.
+Qed.*)
+
+Lemma body_kfree1_freelist: semax_body Vprog Gprog f_kfree1 kfree1_freelist_spec.
+Proof. start_function. Intros. repeat forward. entailer. 
+       induction n. 
+       - assert (original_freelist_pointer = nullval). {
+            rewrite <- H2; auto.
+         }
+         rewrite H8. unfold freelistrep. Exists nullval. entailer.
+      - unfold freelistrep. Intros next_orig. Exists original_freelist_pointer. entailer.
+         Exists next_orig. entailer. fold freelistrep. entailer!.
 Qed.
 
-Lemma body_freerange_no_loop_no_add: semax_body Vprog Gprog f_freerange_no_loop_no_add freerange_no_loop_no_add_spec.
+(*Lemma body_freerange_no_loop_no_add: semax_body Vprog Gprog f_freerange_no_loop_no_add freerange_no_loop_no_add_spec.
 Proof. start_function.
 forward_if. 
    -apply andp_left1. entailer!.
@@ -416,7 +770,7 @@ forward_if.
         unfold pointer_comparison in e1.
         rewrite e2 in e1. inversion e1.
       + apply andp_left2. entailer!.
-Qed.
+Qed.*)
 
 Lemma body_freerange_no_loop_no_add_1: semax_body Vprog Gprog f_freerange_no_loop_no_add_1 freerange_no_loop_no_add_1_spec.
 Proof. start_function.
@@ -478,9 +832,9 @@ forward_while
     temp _pa_end (Vptr b_n_init p_n_init)
     )
    SEP (denote_tc_test_order ((Vptr b_s_init (Ptrofs.add p_s_tmp (Ptrofs.repr (PGSIZE))))) (Vptr b_n_init p_n_init))).
-   - repeat EExists; entailer.
-   - entailer!. entailer.
-   - repeat forward. 
+   - repeat EExists; entailer. (* the precondition (of the whole loop) implies the loop invariant *)
+   - entailer!. entailer. (* the loop-condition expression type-checks (i.e., guarantees to evalu- ate successfully) *)
+   - repeat forward. (* the postcondition of the loop body implies the loop invariant *)
     +entailer!. apply c_tmp_bounds with (p_s_init:=p_s_init) (p_s_tmp:=p_s_tmp) (p_n_init:=p_n_init); try rep_lia. 
     + Exists (c_tmp + 1, Ptrofs.add p_s_tmp (Ptrofs.repr PGSIZE)). entailer!.
         * split.
@@ -494,9 +848,8 @@ forward_while
         * entailer!. specialize (H0 p_s_tmp); apply H0. split_lia.
         destruct H1 as [H11 [H12 [H13 H14]]]. rewrite H11. apply Zle_left_rev.
         assert ( Ptrofs.unsigned p_s_init + c_tmp * PGSIZE + - Ptrofs.unsigned p_s_init =  Ptrofs.unsigned p_s_init + - Ptrofs.unsigned p_s_init + c_tmp * PGSIZE) by rep_lia. 
-        rewrite H1. assert (Ptrofs.unsigned p_s_init + - Ptrofs.unsigned p_s_init = 0) by rep_lia.
-        apply Z.add_nonneg_nonneg; unfold PGSIZE; rep_lia.
-    - forward. Exists c_tmp p_s_tmp. entailer!. split_lia.
+        rewrite H1. le_sub_self_add_and_solve.
+    - forward. Exists c_tmp p_s_tmp. entailer!. split_lia. (* he loop invariant (and negation of the loop condition) is a strong enough precondition to prove the MORE-COMMANDS after the loop *)
         apply typed_false_offset_val_leq with (b_s_init:=b_s_init) (b_n_init:=b_n_init); try rep_lia; unfold PGSIZE; try rep_lia; auto.
 Qed.
 
@@ -506,23 +859,164 @@ Qed.
 Lemma body_freerange_while_loop_spec: semax_body Vprog Gprog f_freerange_while_loop freerange_while_loop_spec.
 Proof. start_function. 
 forward_while
- (EX c_tmp: Z, EX p_s_tmp:ptrofs,
+ (EX c_tmp: Z, EX p_s_tmp:ptrofs, EX head:val,
    PROP  (
     Ptrofs.unsigned p_s_tmp = Z.add (Ptrofs.unsigned p_s_init) (Z.mul c_tmp PGSIZE) /\ 
     0 <= c_tmp /\
     c_tmp <= Int.max_signed /\
-    Ptrofs.unsigned p_s_tmp <= Ptrofs.unsigned p_n_init
+    Ptrofs.unsigned p_s_tmp <= Ptrofs.unsigned p_n_init /\
+    (head = original_freelist_pointer \/ head = (Vptr b_s_init p_s_tmp))
    )
    LOCAL (
-    temp _c (Vint (Int.repr c_tmp));
-    temp _pa_start (Vptr b_s_init p_s_tmp);
-    temp _pa_end (Vptr b_n_init p_n_init)
-    )
-   SEP (denote_tc_test_order ((Vptr b_s_init (Ptrofs.add p_s_tmp (Ptrofs.repr (PGSIZE))))) (Vptr b_n_init p_n_init))).
-   - repeat EExists; entailer.
-   - entailer!. entailer.
+      gvars gv;
+      temp _pa_start (Vptr b_s_init p_s_tmp);
+      temp _pa_end (Vptr b_n_init p_n_init)
+    ) 
+   SEP (
+      denote_tc_test_order ((Vptr b_s_init (Ptrofs.add p_s_tmp (Ptrofs.repr (PGSIZE))))) (Vptr b_n_init p_n_init) &&
+      (*(!! forall p_s_tmp, Ptrofs.unsigned p_s_init <= Ptrofs.unsigned p_s_tmp <= Ptrofs.unsigned p_n_init -> 
+             malloc_compatible (sizeof t_run) (Vptr b_s_init p_s_tmp)) &&*)
+      (freelistrep sh (Nat.add (Z.to_nat c_tmp) n) (head) *
+      available_range sh (Vptr b_s_init p_s_tmp) (Vptr b_n_init p_n_init) (compute_c (Vptr b_s_init p_s_tmp) (Vptr b_n_init p_n_init) PGSIZE) *
+      data_at sh t_struct_kmem (Vint (Int.repr xx), head) (gv _kmem)
+        (* (data_at sh (t_run) nullval (Vptr b_s_init (Ptrofs.add p_s_tmp (Ptrofs.repr PGSIZE)))) *
+         (data_at sh t_struct_kmem (Vint (Int.repr xx), (head)) (gv _kmem))*)
+        (* I havent written anything baout freelistrep nor data_at with the kmem.. *)
+      )
+      )
+  )%assert.
+  - Exists 0 p_s_init original_freelist_pointer. entailer. (* admit begins here*)
+  (*apply andp_right.
+  + apply andp_left1; entailer. 
+  + apply andp_left2; entailer. replace (Nat.add (Z.to_nat 0) n) with (n); try rep_lia. entailer!.
+  entailer!. apply H1; split_lia.
+  + apply andp_right.
+     * apply andp_left1. entailer.
+     * apply andp_left2. 
+        repeat (apply sepcon_derives); entailer.
+        apply H2; split_lia.*)
+   - entailer. apply andp_left1. entailer.
+   -  forward_call (sh, (Vptr b_s_init p_s_tmp), head, xx, gv, (Nat.add (Z.to_nat c_tmp) n), PGSIZE).
+      2: { destruct H as [H1 [H2 [H3 [H4 H5]]]]; split; auto.
+            destruct H0 as [H01 [H02 [H03 [H04 H05]]]]; destruct H05; subst; auto.
+            unfold is_pointer_or_null; auto.
+       }
+      + apply andp_left2. entailer!.
+
+         jeg er i gang med at bevise, at pre condition fører til pre condition for kfree1. måske skal jeg kigge på kfree1 igen.. jeg har alelerede prøvet, men lige nu virker den som om, at den kun vil have en.
+         Jeg ved det ikke.. 
+         unfold available_range. unfold available. 
+
+         destruct (sameblock (Vptr b_s_init p_s_tmp) (Vptr b_n_init p_n_init)) eqn:eb.
+         * apply sameblock_true in eb. subst. entailer!.
+            
+         
+         fold available.
+      (* I have to prove that what I have can give the pre-conditions for kfree..*)
+      + entailer. apply andp_left2.
+         unfold available_range; unfold available.
+         destruct (sameblock (Vptr b_s_init p_s_tmp) (Vptr b_n_init p_n_init)) eqn:eb; unfold sameblock in eb; destruct (peq b_s_init b_n_init) eqn:eb1; auto_contradict.
+         * subst. admit.
+         * 
+
+      apply andp_right.
+         * entailer!. admit.
+         * entailer!. unfold available_range; unfold available.
+            destruct (sameblock (Vptr b_s_init p_s_tmp) (Vptr b_n_init p_n_init)) eqn:eb; auto_contradict.
+      
+      2: {  }
+      
+         * entailer!. admit.
+         * entailer.
+
+
+      forward_call (sh, (Vptr b_s_init (Ptrofs.add p_s_tmp (Ptrofs.mul (Ptrofs.repr (Ctypes.sizeof tschar)) (ptrofs_of_int Signed (Int.repr PGSIZE))))), (Vptr b_s_init p_s_tmp), xx, gv, n).
+
+
+  Admitted.
+
+
+
+
+
+
+
+  (* without availabel range.. *)
+
+Lemma body_freerange_while_loop_spec: semax_body Vprog Gprog f_freerange_while_loop freerange_while_loop_spec.
+Proof. start_function. 
+forward_while
+ (EX c_tmp: Z, EX p_s_tmp:ptrofs, EX head:val,
+   PROP  (
+    Ptrofs.unsigned p_s_tmp = Z.add (Ptrofs.unsigned p_s_init) (Z.mul c_tmp PGSIZE) /\ 
+    0 <= c_tmp /\
+    c_tmp <= Int.max_signed /\
+    Ptrofs.unsigned p_s_tmp <= Ptrofs.unsigned p_n_init /\
+
+    malloc_compatible (sizeof t_run) (Vptr b_s_init p_s_tmp) 
+   )
+   LOCAL (
+      gvars gv;
+      temp _pa_start (Vptr b_s_init p_s_tmp);
+      temp _pa_end (Vptr b_n_init p_n_init)
+    ) 
+   SEP (
+      denote_tc_test_order ((Vptr b_s_init (Ptrofs.add p_s_tmp (Ptrofs.repr (PGSIZE))))) (Vptr b_n_init p_n_init) &&
+      (!! forall p_s_tmp, Ptrofs.unsigned p_s_init <= Ptrofs.unsigned p_s_tmp <= Ptrofs.unsigned p_n_init -> 
+             malloc_compatible (sizeof t_run) (Vptr b_s_init p_s_tmp)) &&
+      (  freelistrep sh (Z.to_nat c_tmp) (head) *
+         (data_at sh (t_run) nullval (Vptr b_s_init (Ptrofs.add p_s_tmp (Ptrofs.repr PGSIZE)))) *
+         (data_at sh t_struct_kmem (Vint (Int.repr xx), (head)) (gv _kmem))
+        (* I havent written anything baout freelistrep nor data_at with the kmem.. *)
+      )
+      )
+  )%assert.
+   - Exists (Z.of_nat n) p_s_init original_freelist_pointer. entailer. (* admit begins here*)
+      apply andp_right.
+      + entailer!. apply H1; split_lia.
+      + apply andp_right.
+         * apply andp_left1. entailer.
+         * apply andp_left2. 
+            repeat (apply sepcon_derives); entailer.
+            apply H2; split_lia.
+   - entailer!. apply andp_left1. entailer.
    - repeat forward. 
-    +entailer!. apply c_tmp_bounds with (p_s_init:=p_s_init) (p_s_tmp:=p_s_tmp) (p_n_init:=p_n_init); try rep_lia. 
+   (* fix free list..*)
+      forward_call (sh, (Vptr b_s_init (Ptrofs.add p_s_tmp (Ptrofs.mul (Ptrofs.repr (Ctypes.sizeof tschar)) (ptrofs_of_int Signed (Int.repr PGSIZE))))), (Vptr b_s_init p_s_tmp), xx, gv, n).
+      + entailer!.
+         * apply H1. split_lia.
+            -- replace (Ptrofs.repr (Int.signed (Int.repr PGSIZE))) with (Ptrofs.repr PGSIZE) by auto.
+               replace (Ptrofs.unsigned (Ptrofs.add p_s_tmp (Ptrofs.repr PGSIZE))) with (Ptrofs.unsigned p_s_tmp + PGSIZE) by (symmetry; ptrofs_add_simpl_PGSIZE).
+               destruct H0 as [H00 H01]; rewrite H00.
+               rewrite ZMicromega.le_0_iff.
+               replace (Ptrofs.unsigned p_s_init + c_tmp * PGSIZE + PGSIZE - Ptrofs.unsigned p_s_init) with (Ptrofs.unsigned p_s_init + - Ptrofs.unsigned p_s_init + c_tmp * PGSIZE + PGSIZE); try rep_lia.
+               le_sub_self_add_and_solve.
+            -- apply typed_true_offset_val_leq with (b_s_init:=b_s_init) (b_n_init :=b_n_init); unfold PGSIZE; auto.
+         * apply andp_left2. entailer!. admit.
+      + destruct H as [H2 [H3 [H4 [H5 H6]]]]; auto.
+      + Exists (c_tmp + 1, Ptrofs.add p_s_tmp (Ptrofs.repr PGSIZE), (Z.to_nat c_tmp),Vptr b_s_init (Ptrofs.add p_s_tmp (Ptrofs.mul (Ptrofs.repr (Ctypes.sizeof tschar)) (ptrofs_of_int Signed (Int.repr PGSIZE))))). 
+        destruct H0 as [H2 [H3 [H4 [H5 H6]]]]; auto; entailer!. 
+         *split; try split; try split; try split; try rep_lia.
+            -- replace (Ptrofs.unsigned (Ptrofs.add p_s_tmp (Ptrofs.repr PGSIZE))) with (Ptrofs.unsigned p_s_tmp + PGSIZE) by (symmetry; ptrofs_add_simpl_PGSIZE).
+               rewrite H2; try rep_lia.
+            -- apply c_tmp_bounds_max with (p_s_init:=p_s_init) (p_s_tmp:=p_s_tmp) (p_n_init:=p_n_init); try rep_lia.
+            -- apply typed_true_offset_val_leq with (b_s_init:=b_s_init) (b_n_init :=b_n_init); unfold PGSIZE; auto.
+            -- apply H1. split_lia.
+               ++ replace (Ptrofs.unsigned (Ptrofs.add p_s_tmp (Ptrofs.repr PGSIZE))) with (Ptrofs.unsigned p_s_tmp + PGSIZE) by (symmetry; ptrofs_add_simpl_PGSIZE).
+                  rewrite H2. 
+                  rewrite ZMicromega.le_0_iff.
+                  replace (Ptrofs.unsigned p_s_init + c_tmp * PGSIZE + PGSIZE - Ptrofs.unsigned p_s_init) with (Ptrofs.unsigned p_s_init + - Ptrofs.unsigned p_s_init + c_tmp * PGSIZE + PGSIZE); try rep_lia.
+                  le_sub_self_add_and_solve.
+               ++ apply typed_true_offset_val_leq with (b_s_init:=b_s_init) (b_n_init :=b_n_init); unfold PGSIZE; auto.
+         * 
+      admit.
+               
+      + destruct H as [H2 [H3 [H4 [H5 H6]]]]; split; auto.
+      + Exists (c_tmp + 1, Ptrofs.add p_s_tmp (Ptrofs.repr PGSIZE), (Z.to_nat c_tmp)). entailer. admit.
+
+
+      (* under er der kode fra forward while.. *)
+   (* +entailer!. apply c_tmp_bounds with (p_s_init:=p_s_init) (p_s_tmp:=p_s_tmp) (p_n_init:=p_n_init); try rep_lia. 
     + Exists (c_tmp + 1, Ptrofs.add p_s_tmp (Ptrofs.repr PGSIZE)). entailer!.
         * split.
          -- destruct H as [H2 [H3 H4]].
@@ -536,7 +1030,7 @@ forward_while
         destruct H1 as [H11 [H12 [H13 H14]]]. rewrite H11. apply Zle_left_rev.
         assert ( Ptrofs.unsigned p_s_init + c_tmp * PGSIZE + - Ptrofs.unsigned p_s_init =  Ptrofs.unsigned p_s_init + - Ptrofs.unsigned p_s_init + c_tmp * PGSIZE) by rep_lia. 
         rewrite H1. assert (Ptrofs.unsigned p_s_init + - Ptrofs.unsigned p_s_init = 0) by rep_lia.
-        apply Z.add_nonneg_nonneg; unfold PGSIZE; rep_lia.
+        apply Z.add_nonneg_nonneg; unfold PGSIZE; rep_lia.*)
     - forward. Exists c_tmp p_s_tmp. entailer!. split_lia.
         apply typed_false_offset_val_leq with (b_s_init:=b_s_init) (b_n_init:=b_n_init); try rep_lia; unfold PGSIZE; try rep_lia; auto.
 Qed.
